@prefix aoi: <https://w3id.org/aoi#> .
@prefix dot: <https://w3id.org/dot#> .
@prefix owl: <http://www.w3.org/2002/07/owl#> .
@prefix rdf: <http://www.w3.org/1999/02/22-rdf-syntax-ns#> .
@prefix xml: <http://www.w3.org/XML/1998/namespace> .
@prefix xsd: <http://www.w3.org/2001/XMLSchema#> .
@prefix foaf: <http://xmlns.com/foaf/0.1/> .
@prefix obda: <https://w3id.org/obda/vocabulary#> .
@prefix rdfs: <http://www.w3.org/2000/01/rdf-schema#> .
@prefix vann: <http://purl.org/vocab/vann/> .
@prefix dcterms: <http://purl.org/dc/terms/> .

<https://w3id.org/aoi> rdf:type owl:Ontology ;
                                  owl:versionIRI <https://w3id.org/aoi/0.2> ;
                                  dcterms:creator [ rdf:type foaf:Person ;
                                                    foaf:name "Al-Hakam Hamdan"
                                                  ] ;
                                  dcterms:description "Auxiliary ontology that defines areas of interests on a component which can be affected by damages(defined in DOT)"@en ;
                                  dcterms:license "https://creativecommons.org/licenses/by/1.0" ;
                                  dcterms:title "Areas of Interests"@en ;
                                  vann:preferredNamespacePrefix "aoi" ;
                                  vann:preferredNamespaceUri "https://w3id.org/aoi#" .

#################################################################
#    Object Properties
#################################################################

###  https://w3id.org/aoi#locates
aoi:locates rdf:type owl:ObjectProperty ;
			rdfs:domain aoi:AreaOfInterest ;
			rdfs:comment "Defines the relationship between an AOI and an Individual, which is somehow topologically connected with a component that has the AOI."@en ;
			rdfs:label "locates"@en .


###  https://w3id.org/aoi#locatesDamage
aoi:locatesDamage rdf:type owl:ObjectProperty ;
				  rdfs:subPropertyOf aoi:locates ;
                   rdfs:domain aoi:AreaOfInterest ;
                   rdfs:range dot:Damage ;
                   rdfs:comment "Defines the relationship between an AOI and a Damage."@en ;
                   rdfs:label "locates Damage"@en .


###  https://w3id.org/aoi#hasAreaOfInterest
aoi:hasAreaOfInterest rdf:type owl:ObjectProperty ;
                      rdfs:range aoi:AreaOfInterest ;
                      owl:propertyChainAxiom ( aoi:hasSide
                                               aoi:hasAreaOfInterest
                                             ) ;
                      rdfs:comment "Defines the relationship between an affected component or structure (e.g. bot:Element) and an AOI."@en ;
                      rdfs:label "has Area of Interest"@en .


###  https://w3id.org/aoi#hasSide
aoi:hasSide rdf:type owl:ObjectProperty ;
                      rdfs:range aoi:ComponentSide ;
                      rdfs:comment "Defines the relationship between a component or structure (e.g. bot:Element) and its side."@en ;
                      rdfs:label "has component side"@en .


#################################################################
#    Classes
#################################################################

###  https://w3id.org/aoi#AreaOfInterest
aoi:AreaOfInterest rdf:type owl:Class ;
                   rdfs:comment "Area of a construction component that is of specific interest, e.g. for assignment of damages"@en ;
                   rdfs:label "Area of Interest (AOI)"@en .


###  https://w3id.org/aoi#ComponentSide
aoi:ComponentSide rdf:type owl:Class ;
                   rdfs:comment "Area of a construction component that represents a specific horizontal side of a component"@en ;
                   rdfs:label "Component Side"@en .


###  https://w3id.org/aoi#Bottom
aoi:Bottom rdf:type owl:Class ;
           rdfs:subClassOf aoi:LowerArea ,
                           aoi:Surface ;
           rdfs:comment "AOI that defines the bottom a construction component based on its local coordinate system. No lower located AOI is allowed."@en ;
           rdfs:label "Bottom"@en .


###  https://w3id.org/aoi#Edge
aoi:Edge rdf:type owl:Class ;
         rdfs:subClassOf aoi:ExteriorArea ;
         rdfs:comment "Defines an interface, where two AOI intersect."@en ;
         rdfs:label "Edge"@en .


###  https://w3id.org/aoi#ExteriorArea
aoi:ExteriorArea rdf:type owl:Class ;
                 rdfs:subClassOf aoi:AreaOfInterest ;
                 owl:disjointWith aoi:InternalArea ;
                 rdfs:comment "AOI that defines the outer areal of a construction component based on its local coordinate system."@en ;
                 rdfs:label "Exterior Area"@en .


###  https://w3id.org/aoi#HorizontalCentralArea
aoi:HorizontalCentralArea rdf:type owl:Class ;
                          rdfs:subClassOf aoi:AreaOfInterest ;
                          owl:disjointWith aoi:PeripheralArea ;
                          rdfs:comment "AOI that defines the horizontal central area of a construction component."@en ;
                          rdfs:label "Horizontal Central Area"@en .


###  https://w3id.org/aoi#InternalArea
aoi:InternalArea rdf:type owl:Class ;
                 rdfs:subClassOf aoi:AreaOfInterest ;
                 rdfs:comment "AOI that defines the inner areal of a construction component based on its local coordinate system."@en ;
                 rdfs:label "Internal Area"@en .


###  https://w3id.org/aoi#LowerArea
aoi:LowerArea rdf:type owl:Class ;
              rdfs:subClassOf aoi:AreaOfInterest ;
              rdfs:comment "AOI that defines the lower area of a construction component based on its local coordinate system."@en ;
              rdfs:label "Lower Area"@en .


###  https://w3id.org/aoi#PeripheralArea
aoi:PeripheralArea rdf:type owl:Class ;
                   rdfs:subClassOf aoi:AreaOfInterest ;
                   rdfs:comment "AOI that defines the peripheral horizontal area of a construction component based on its local coordinate system."@en ;
                   rdfs:label "Peripheral Area"@en .


###  https://w3id.org/aoi#Periphery
aoi:Periphery rdf:type owl:Class ;
              rdfs:subClassOf aoi:PeripheralArea ,
                              aoi:Surface ;
              rdfs:comment "AOI that defines a periphery of a construction component based on its local coordinate system."@en ;
              rdfs:label "Periphery"@en .


###  https://w3id.org/aoi#Surface
aoi:Surface rdf:type owl:Class ;
            rdfs:subClassOf aoi:ExteriorArea ;
            rdfs:comment "AOI that defines the vertical central area of a construction component based on its local coordinate system."@en ;
            rdfs:label "Surface"@en .


###  https://w3id.org/aoi#Top
aoi:Top rdf:type owl:Class ;
        rdfs:subClassOf aoi:Surface ,
                        aoi:UpperArea ;
        rdfs:comment "AOI that defines the top a construction component based on its local coordinate system. No higher located AOI is allowed."@en ;
        rdfs:label "Top"@en .


###  https://w3id.org/aoi#UpperArea
aoi:UpperArea rdf:type owl:Class ;
              rdfs:subClassOf aoi:AreaOfInterest ;
              rdfs:comment "AOI that defines the upper area of a construction component based on its local coordinate system."@en ;
              rdfs:label "Upper Area"@en .


###  https://w3id.org/aoi#VerticalCentralArea
aoi:VerticalCentralArea rdf:type owl:Class ;
                        rdfs:subClassOf aoi:AreaOfInterest ;
                        rdfs:comment "AOI that defines the vertical central area of a construction component based on its local coordinate system."@en ;
                        rdfs:label "Vertical Central Area"@en .

#################################################################
#    General axioms
#################################################################

[ rdf:type owl:AllDisjointClasses ;
   owl:members ( aoi:LowerArea
                 aoi:UpperArea
                 aoi:VerticalCentralArea
               )
 ] .
